Add annotations to ch3 demo files

demos/ch03/nim_v2.dfy
@@ -8,31 +8,63 @@ ghost predicate Init(v: Variables) {
   && v.turn.P1? // syntax
 }
 
-datatype Step = TurnStep(take: nat, p: nat)
+// We re-write the v1 version using Jay Normal Form, putting all non-determinism
+// into this Step datatype.
+// DEMO: added NoOp step live
+datatype Step =
+  | TurnStep(take: nat, p: nat)
+  | NoOpStep()
 
 ghost predicate Turn(v: Variables, v': Variables, step: Step)
-  requires step.TurnStep? // syntax
+  requires step.TurnStep? // syntax for requiring this be a TurnStep
 {
-  var p := step.p; // syntax
+  // syntax: var in a function/predicate is immutable; it's just a shorthand to
+  // make definitions more readable.
+  // step.p accesses the p field of TurnStep. This is only legal because
+  // `requires step.TurnStep?` ensures that constructor was used - NoOpStep
+  // wouldn't have such a field.
+  var p := step.p;
   var take := step.take;
   && p < |v.piles|
   && take <= v.piles[p]
   && v'.piles == v.piles[p := v.piles[p] - take]
+     // DEMO: the same bug is here, but it'll be easier to debug
+}
+
+ghost predicate NoOp(v: Variables, v': Variables, step: Step)
+  requires step.NoOpStep?
+{
+  v' == v
 }
 
 // nearly boilerplate (just gather up all transitions)
 ghost predicate NextStep(v: Variables,  v': Variables, step: Step) {
   match step {
     case TurnStep(_, _) => Turn(v, v', step)
+    case NoOpStep() => NoOp(v, v', step)
   }
 }
 
 // boilerplate - always the same
-lemma NextStepDeterminsticGivenStep(v: Variables, v': Variables, v'': Variables, step: Step)
+lemma NextStepDeterministicGivenStep(v: Variables, v': Variables, v'': Variables, step: Step)
   requires NextStep(v, v', step)
   requires NextStep(v, v'', step)
   ensures v' == v''
 {
+  // DEMO: doesn't go through! let's debug it
+  match step {
+    case TurnStep(_, _) => {
+      // DEMO: what part of variables isn't being specified deterministically?
+      assert v'.piles == v''.piles;
+      // this fails, at this point hopefully we realize we forgot to specify
+      // turn entirely (if not, we'd add more assertions)
+      assert v'.turn == v''.turn;
+    }
+    case NoOpStep() => {
+      // no error here
+      return;
+    }
+  }
 }
 
 // boilerplate - always the same
