demos/ch03/search_specs.dfy
@@ -1,17 +1,31 @@
+// In this file we'll explore some specifications for binary search. We won't
+// have a definition, so we'll just write predicates that capture the
+// BinarySearch ensures clause, and then reason about those predicates on their
+// own.
+
 ghost predicate IsSorted(s:seq<int>) {
   forall i:nat, j:nat | i < j < |s| :: s[i] <= s[j]
 }
 
 ghost predicate SearchIndex1(haystack: seq<int>, needle: int, i: nat)
 {
+  // DEMO: some people tried to write predicates that morally looked like the
+  // comments. To make this plan actually work and handle all edge cases
+  // requires a much more complicated definition, too complicated for a
+  // specification for my taste (it's very easy to get this wrong).
   // && haystack[i-1] < needle
   // && haystack[i] <= needle
   && (i == 0 || (i-1 < |haystack| ==> haystack[i-1] < needle))
   && (i < |haystack| ==> haystack[i] >= needle)
   && (i == |haystack| ==> forall j:nat | j < |haystack| :: haystack[j] < needle)
+     // DEMO: add this back to make SearchIndex1 deterministic
      // && i <= |haystack|
 }
 
+// One desirable property for binary search is to have a deterministic
+// specification. This is especially the case for the assignment because it
+// clarifies that if the needle is found multiple times, the lowest index should
+// be returned.
 lemma SearchIndex1Deterministic(haystack: seq<int>, needle: int, i1: nat, i2: nat)
   requires IsSorted(haystack)
   requires SearchIndex1(haystack, needle, i1)
@@ -19,6 +33,8 @@ lemma SearchIndex1Deterministic(haystack: seq<int>, needle: int, i1: nat, i2: na
   ensures i1 == i2
 {}
 
+// This is what I find a more elegant approach to capturing the same idea as the
+// first attempt.
 ghost predicate SearchIndex2(haystack: seq<int>, needle: int, i: nat)
 {
   && (forall j:nat | j < i < |haystack| :: haystack[j] <= needle)
@@ -34,18 +50,29 @@ lemma SearchIndex2Deterministic(haystack: seq<int>, needle: int, i1: nat, i2: na
 {
 }
 
+// DEMO: there's a bug in the above, because it says haystack[j] <= needle it
+// allows any index that contains the needle, not just the smallest one.
+//
+// Here we prove the opposite of SearchIndex2Deterministic. Whereas that lemma
+// is a proof for all values of haystack, needle, i1, and i2, here we show there
+// _exists_ a counter-example, returning it from the lemma.
 lemma SeachIndex2NonDet() returns (haystack: seq<int>, needle: int, i1: nat, i2: nat)
   ensures IsSorted(haystack)
   ensures SearchIndex2(haystack, needle, i1)
   ensures SearchIndex2(haystack, needle, i2)
   ensures i1 != i2
 {
+  // the crux is that the needle appears twice
   haystack := [1, 2, 2, 3];
+  assert IsSorted(haystack);
   needle := 2;
   i1 := 1;
   i2 := 2;
 }
 
+// Here we fix that bug and also add another clause about exactly what happens
+// if i == |haystack|. This is enough to make it deterministic, although as you
+// can see below that proof wasn't so simple.
 ghost predicate SearchIndex3(haystack: seq<int>, needle: int, i: nat)
 {
   && (forall j:nat | j < i < |haystack| :: haystack[j] < needle)
